cleaning in examples

theories/iris/examples/segstack/function/segstack_push.v
@@ -35,8 +35,8 @@ Section stack.
   1 (input)     i32 value to be pushed
   2             temporary variable storing the new address of the stack top pointer
 *)
-    Definition push_op :=
-      is_full_op ++ 
+    Definition push :=
+      is_full ++ 
      [
        BI_if (Tf [] []) [BI_unreachable] [];
        BI_get_local 0 ;
@@ -53,14 +53,11 @@ Section stack.
        BI_segstore T_i32 
       ].
         
-    Definition push :=
-      (*validate_stack 0 ++ validate_stack_bound 0 ++*) push_op.
-    
   End code.
 
   Section specs.
     
-    Lemma spec_push_op f0 (v: handle) (a : i32) s E :
+    Lemma spec_push f0 (v: handle) (a : i32) s E :
       ⊢ {{{ 
            ⌜ f0.(f_locs) !! 0 = Some (value_of_handle v) ⌝
           ∗ ⌜ f0.(f_locs) !! 1 = Some (VAL_int32 a) ⌝ 
@@ -68,7 +65,7 @@ Section stack.
           ∗ ⌜ (N.of_nat (length s) < two14 - 1)%N ⌝
           ∗ isStack v s
           ∗ ↪[frame] f0 }}}
-        to_e_list push_op @ E
+        to_e_list push @ E
         {{{ w, ⌜ w = immV [] ⌝ ∗
                        isStack v (a :: s) ∗
                        ∃ f1, ↪[frame] f1 ∗ ⌜ f_inst f0 = f_inst f1 ⌝ }}}. 
@@ -80,7 +77,7 @@ Section stack.
       rewrite (separate4 (AI_basic _)).
       iApply wp_seq.
       iSplitR; last iSplitL "Hf Hstack".
-      2: { iApply (spec_is_full_op with "[$Hf $Hstack] []") => //.
+      2: { iApply (spec_is_full with "[$Hf $Hstack] []") => //.
            iIntros (w) "H".
            by iApply "H".
       }
@@ -370,200 +367,10 @@ Section stack.
         lia. rewrite H.  done.
     Qed.
 
-    (*
-    Lemma spec_push f0 n (v: N) (a : i32) s E :
-      ⊢ {{{ ⌜ f0.(f_inst).(inst_memory) !! 0 = Some n ⌝
-          ∗ ⌜ f0.(f_locs) !! 0 = Some (value_of_uint v) ⌝
-          ∗ ⌜ f0.(f_locs) !! 1 = Some (VAL_int32 a) ⌝ 
-          ∗ ⌜ length f0.(f_locs) >= 3 ⌝
-         ∗ ⌜ (N.of_nat (length s) < two14 - 1)%N ⌝
-          ∗ isStack v s n
-          ∗ ↪[frame] f0 }}}
-        to_e_list push @ E
-        {{{ w, ⌜ w = immV [] ⌝ ∗
-                       isStack v (a :: s) n ∗
-                       ∃ f1, ↪[frame] f1 ∗ ⌜ f_inst f0 = f_inst f1 ⌝ }}}. 
-    Proof.
-      iIntros "!>" (Φ) "(%Hinst & %Hlocv & %Hloca & %Hlocs & %Hlens & Hstack & Hf) HΦ" => /=.
-      
-      rewrite separate4.
-      iApply wp_seq.
-      instantiate (1 := λ x,  (⌜ x = immV [] ⌝ ∗ isStack v s n ∗ ↪[frame] f0)%I).
-      iSplitR; first by iIntros "(%H & _)".
-      iSplitL "Hstack Hf"; first by iApply (is_stack_valid with "[$Hstack $Hf]").
-      
-      iIntros (w) "(-> & Hstack & Hf) /=".
-      rewrite separate3.
-      iApply wp_seq.
-      instantiate (1 := λ x,  (⌜ x = immV [] ⌝ ∗ isStack v s n ∗ ↪[frame] f0)%I).
-      iSplitR; first by iIntros "(%H & _)".
-      iSplitL "Hstack Hf"; first by iApply (is_stack_bound_valid with "[$Hstack $Hf]").
-      
-      iIntros (w) "(-> & Hstack & Hf) /=".
-      iApply (spec_push_op with "[$Hf $Hstack] [$]").
-      auto.
-    Qed. *)
       
   End specs.
 
 
-  Section valid.
-    Context `{!logrel_na_invs Σ, !cinvG Σ, cancelg: cancelG Σ}.
-    Set Bullet Behavior "Strict Subproofs".
-(*
-    Lemma valid_push m t funcs :
-    let i0 := {| inst_types := [Tf [] [T_i32]; Tf [T_i32] [T_i32]; Tf [T_i32; T_i32] []];
-                     inst_funcs := funcs;
-                     inst_tab := [t];
-                     inst_memory := [m];
-                     inst_globs := []
-              |} in
-    na_inv logrel_nais stkN (stackModuleInv (λ (a : N) (b : seq.seq i32), isStack a b m) (λ n : nat, N.of_nat m↦[wmlength]N.of_nat n)) -∗
-    interp_closure_native i0 [T_i32;T_i32] [] [T_i32] (to_e_list push) [].
-  Proof.
-    iIntros "#Hstk".
-    iIntros (vcs f) "#Hv Hown Hf".
-    iIntros (LI HLI%lfilled_Ind_Equivalent);inversion HLI;inversion H8;subst;simpl.
-    iApply (wp_frame_bind with "[$]");auto.
-    iIntros "Hf".
-    match goal with | |- context [ [AI_label _ _ ?l] ] => set (e:=l) end.
-    build_ctx e.
-    iApply wp_label_bind.
-    subst e.
-    iDestruct "Hv" as "[%Hcontr|Hws]";[done|iDestruct "Hws" as (ws) "[%Heq Hws]"].
-    iDestruct (big_sepL2_length with "Hws") as %Hlen. inversion Heq;subst.
-    destruct ws as [|w0 ws];[done|destruct ws as [|w1 ws];[done|destruct ws as [|w2 ws];[|done]]].
-    iSimpl in "Hws".
-    iDestruct "Hws" as "[Hw0 [Hw1 _]]".
-    iDestruct "Hw0" as (z0) "->".
-    iDestruct "Hw1" as (z1) "->".
-    pose proof (value_of_uint_repr z0) as [v ->]. iSimpl in "Hf".
-    take_drop_app_rewrite (length (validate_stack 1)).
-
-    match goal with | |- context [ (WP ?e @ _; _ {{ _ }} )%I ] => set (e0:=e) end.
-    match goal with | |- context [ (↪[frame] ?f0)%I ] => set (f':=f0) end.
-    build_ctx e0. subst e0.
-    iApply wp_seq_can_trap_ctx.
-    instantiate (1:=(λ f0, ⌜f0 = f'⌝ ∗ na_own logrel_nais ⊤)%I).
-    iFrame "Hf".
-    iSplitR;[|iSplitR;[|iSplitL]];cycle 1.
-    - iIntros (f0) "(Hf & -> & Hown)".
-      deconstruct_ctx.
-      iApply (wp_wand _ _ _ (λ v, ⌜v = trapV⌝ ∗ _)%I with "[Hf]").
-      iApply (wp_label_trap with "Hf");auto.
-      iIntros (v0) "[-> Hf]". iExists _. iFrame.
-      iIntros "Hf".
-      iApply (wp_frame_trap with "Hf").
-      iNext. iLeft. iLeft. auto.
-    - iIntros "Hf". iFrame.
-      iApply (wp_wand with "[Hf]").
-      iApply check_stack_valid;iFrame;subst;eauto.
-      iIntros (v0) "[$ HH]". eauto.
-    - subst f'. iIntros (w f0) "([-> %Hdiv] & Hf & -> & Hown) /=".
-      deconstruct_ctx.
-      take_drop_app_rewrite (length (validate_stack_bound 0)).
-      iApply fupd_wp.
-      iMod (na_inv_acc with "Hstk Hown") as "(>Hstkres & Hown & Hcls)";[solve_ndisj..|].
-      iModIntro.
-      iDestruct "Hstkres" as (l Hmul) "[Hlen Hstkres]".
-      iDestruct "Hstkres" as (l' Hmultiple) "Hl'".
-      match goal with | |- context [ (WP ?e @ _; _ {{ _ }} )%I ] => set (e0:=e) end.
-      match goal with | |- context [ (↪[frame] ?f0)%I ] => set (f':=f0) end.
-      match goal with | |- context [ (?P ={⊤}=∗ ?Q)%I ] => set (CLS:=(P ={⊤}=∗ Q)%I) end.
-      
-      set (k:=Wasm_int.N_of_uint i32m ((Wasm_int.int_of_Z i32m (Z.of_N v)))).
-      destruct (decide (k < N.of_nat l)%N).
-      + apply div_mod_i32 in Hdiv as Hdiv'.
-        eapply multiples_upto_in in Hmultiple as Hin;[..|apply Hdiv'];[|lia].
-        apply elem_of_list_lookup_1 in Hin as [i Hi].
-        iDestruct (big_sepL_lookup_acc with "Hl'") as "[Hv Hl']";[eauto|].
-        iDestruct "Hv" as (stk) "Hv".
-        iApply (wp_seq _ _ _ (λ v, ⌜v = immV []⌝ ∗ _)%I).
-        iSplitR;[by iIntros "[%Hcontr _]"|].
-        iSplitL "Hf Hv".
-        { iApply is_stack_bound_valid. iFrame "Hf Hv". iSplit;auto.
-          iPureIntro. subst f'. simpl. unfold value_of_uint.
-          f_equal. f_equal. apply int_of_Z_mod. }
-        iIntros (w) "(-> & Hstack & Hf) /=".
-        destruct (decide (N.of_nat (length stk) < two14 - 1)%N).
-        * iApply (spec_push_op with "[$Hstack $Hf]").
-          { repeat iSplit;auto. subst f';simpl. iPureIntro.
-            unfold value_of_uint. f_equal. f_equal. apply int_of_Z_mod. }
-          iIntros (w) "[-> [Hstack Hf]]".
-          iDestruct "Hf" as (f1) "[Hf %Hfeq]".
-          iDestruct ("Hl'" with "[Hstack]") as "Hl'".
-          { iExists _. iFrame. }
-          deconstruct_ctx.
-          iApply fupd_wp.
-          iMod ("Hcls" with "[Hlen Hl' $Hown]") as "Hown".
-          { iExists _. iFrame. iNext. iSplit;auto. }
-          iModIntro.
-          iApply (wp_wand _ _ _ (λ v, ⌜v = immV []⌝ ∗ _)%I with "[Hf]").
-          iApply (wp_label_value with "Hf");eauto.
-          iIntros (v0) "[-> Hf]".
-          iExists _. iFrame.
-          iIntros "Hf".
-          iApply (wp_frame_value with "Hf");eauto.
-          iNext. iLeft. iRight. iExists []. simpl. done.
-        * iDestruct (stack_pure with "Hstack") as "(_ & _ & %Hstkbound & Hstack)".
-          take_drop_app_rewrite (length (is_full_op)).
-          iApply wp_seq.
-          iSplitR;[|iSplitL "Hf Hstack"];cycle 1.
-          { iApply (spec_is_full_op with "[$Hf $Hstack]").
-            - repeat iSplit;auto.
-              iPureIntro. subst f';simpl. unfold value_of_uint.
-              f_equal. f_equal. apply int_of_Z_mod.
-            - iIntros (w) "H". iExact "H". }
-          2: iIntros "H";by iDestruct "H" as (? ?) "_".
-          iIntros (w) "H".
-          iDestruct "H" as (k0) "(-> & Hstack & [[-> %Hcond]|[-> %Hcond]] & Hf)";[|lia].
-          simpl.
-          iDestruct ("Hl'" with "[Hstack]") as "Hl'".
-          { iExists _. iFrame. }
-          iApply fupd_wp.
-          iMod ("Hcls" with "[Hlen Hl' $Hown]") as "Hown".
-          { iExists _. iFrame. iNext. iSplit;auto. }
-          iModIntro.
-          take_drop_app_rewrite 2.
-          iApply (wp_wand _ _ _ (λ v, ⌜v = trapV⌝ ∗ _)%I with "[Hf]").
-          iApply wp_seq_trap. iFrame.
-          iIntros "Hf". iApply (wp_if_true with "[$]");auto.
-          iNext. iIntros "Hf".
-          take_drop_app_rewrite 0.
-          iApply (wp_block with "[$]");auto.
-          iNext. iIntros "Hf".
-          build_ctx [AI_basic BI_unreachable].
-          take_drop_app_rewrite 1.
-          iApply wp_seq_trap_ctx. iFrame. iIntros "Hf".
-          iApply (wp_unreachable with "[$]"). auto.
-          iIntros (v') "[-> Hf]".
-          deconstruct_ctx.
-          iApply (wp_wand _ _ _ (λ v, ⌜v = trapV⌝ ∗ _)%I with "[Hf]").
-          iApply (wp_label_trap with "[$]");eauto.
-          iIntros (v0) "[-> Hf]".
-          iExists _. iFrame. iIntros "Hf".
-          iApply (wp_frame_trap with "[$]").
-          iNext. iLeft. iLeft. auto.          
-      + iApply (wp_wand with "[Hlen Hf]").
-        iApply (fail_stack_bound_valid with "[$Hlen $Hf]").
-        eauto.
-        iIntros (v0) "(-> & Hlen & Hf)".
-        deconstruct_ctx.
-        iApply fupd_wp.
-        iMod ("Hcls" with "[$Hown Hl' Hlen]") as "Hown".
-        { iNext. iExists _. iFrame. auto. }
-        iModIntro.
-        iApply (wp_wand _ _ _ (λ v, ⌜v = trapV⌝ ∗ _)%I with "[Hf]").
-        iApply (wp_label_trap with "Hf");eauto.
-        iIntros (v0) "[-> Hf]".
-        iExists _. iFrame. iIntros "Hf".
-        iApply (wp_frame_trap with "[$]").
-        iNext. iLeft. iLeft. auto.
-    - iIntros "[%Hcontr _]";done.
-  Qed.
-*)
-    
-  End valid.
 
 End stack.    
 
